---
date:   2022-08-26 00
---
* Bernoulli 不等式：{::nomarkdown}$ n \geqslant 2, \forall i \in \left[1, n\right] \cdot \left(x_i > - 1 \land x_1x_i > 0\right) \Rightarrow \prod\limits_{i = 1}^n \left(1 + x_i\right) > 1 + \sum\limits_{i = 1}^n x_i ${:/}

* {::nomarkdown}$ \left(1 + \frac{1}{n}\right)^n \uparrow, \left(1 + \frac{1}{n}\right)^{n + 1} \downarrow ${:/}

  {::nomarkdown}\begin{flalign} \label{1} \Leftarrow \forall a, b > 0 \land a \neq b, n \in \N^* \cdot a^{n + 1} > \left(\left(n + 1\right)a - nb\right)b^n & & \end{flalign}{:/}

  {::nomarkdown}$ \Leftrightarrow \forall a > b > 0, n \in \N^* \cdot \left(a - b\right)\left(n + 1\right)b^n < a^{n + 1} - b^{n + 1} < \left(a - b\right)\left(n + 1\right)a^n ${:/}

  （{::nomarkdown}$ \Leftarrow ${:/} Bernoulli 不等式）

* {::nomarkdown}$ A \geqslant G ${:/}

  * {::nomarkdown}$ \Leftarrow n\left(\frac{A}{G} - 1\right) = \sum\limits_{i = 1}^n \int\limits_{a_i}^G \left(\frac{1}{t} - \frac{1}{G}\right) \d t \geqslant 0 ${:/}

  * {::nomarkdown}$ \Leftarrow ${:/} 排序不等式

  * {::nomarkdown}$ \Leftarrow ${:/} Jensen 不等式

  * {::nomarkdown}$ \Leftarrow ${:/} Bernoulli 不等式 {::nomarkdown}$ \eqref{1} ${:/}

## 探究题

### 1.

设 {::nomarkdown}$ c = a - b > 0 ${:/}

由均值不等式，{::nomarkdown}$ 原式 = b + c + \frac{1}{bc} \geqslant 3\sqrt[3]{1} \quad \left(取等 \Leftrightarrow b = c = 1\right) ${:/}

### 2.

设 {::nomarkdown}$ x = \sin^3 \alpha, y = \sin^3 \beta, z = \sin^3 \gamma \in \left(0, 1\right), x + y + z = 1 ${:/}

{::nomarkdown}$ f\left(x\right) := \frac{x^\frac{2}{3}}{1 - x^\frac{2}{3}} \quad \left(x \in \left(0, 1\right)\right) ${:/}

{::nomarkdown}$ x \in \left(0, 1\right) ${:/} 时，由均值不等式，{::nomarkdown}$ x\left(1 - x^2\right) = \sqrt{\frac{\left(2x^2\right)\left(1 - x^2\right)\left(1 - x^2\right)}{2}} \leqslant \sqrt{\frac{\left(\frac{2}{3}\right)^3}{2}} = \frac{2}{3\sqrt{3}} ${:/}

{::nomarkdown}$ \Rightarrow f\left(x\right) = \frac{x}{x^{\frac{1}{3}}\left(1 - x^{\frac{2}{3}}\right)} \geqslant \frac{3}{2}\sqrt{3}x ${:/}

{::nomarkdown}$ \tan^2 \alpha = \frac{\sin^2 \alpha}{1 - \sin^2 \alpha} = f\left(x\right) ${:/}

故 {::nomarkdown}$ \text{LHS} = f\left(x\right) + f\left(y\right) + f\left(z\right) \geqslant \frac{3}{2}\sqrt{3}\left(x + y + z\right) = \text{RHS} ${:/}

### 3.

{::nomarkdown}$ n = 1 ${:/} 时，成立

{::nomarkdown}$ n > 1 ${:/} 时，设 {::nomarkdown}$ f\left(x\right) = x^n \quad \left(x > 0\right), f''\left(x\right) = n\left(n - 1\right)x^{n - 2} > 0 ${:/}

故由琴生不等式，{::nomarkdown}$ \frac{\text{LHS}}{2} = \frac{f\left(x\right) + f\left(y\right)}{2} \geqslant f\left(\frac{x + y}{2}\right) = \left(\frac{1}{2}\right)^n ${:/}，故成立

### 4.

设 {::nomarkdown}$ i_1, i_2, \cdots, i_n ${:/} 为 {::nomarkdown}$ 1, 2, \cdots, n ${:/} 的一个排列，且 {::nomarkdown}$ x_{i_1} < x_{i_2} < \cdots < x_{i_n} ${:/}

{::nomarkdown}$ x_1, x_2, \cdots, x_n ${:/} 互不相同，故 {::nomarkdown}$ \forall k \in \left[1, n\right] \cdot x_{i_k} \geqslant k ${:/}

由排序不等式，{::nomarkdown}$ \sum\limits_{k = 1}^n x_k\frac{1}{k^2} \geqslant \sum\limits_{k = 1}^n x_{i_k}\frac{1}{k^2} \geqslant \sum\limits_{k = 1}^n \frac{1}{k} ${:/}

### 5.

{::nomarkdown}$ \Leftrightarrow x^4y^2 + x^2y^4 \geqslant 2x^3y^3 \Leftrightarrow \left(xy\right)^2\left(x - y\right)^2 \geqslant 0 ${:/}

