## 探究题

### 1.

设原坐标系中 {::nomarkdown}$ \left(x, y\right) ${:/} 在原坐标系逆时针旋转 {::nomarkdown}$ \frac{\pi}{4} ${:/} 所得坐标系中为 {::nomarkdown}$ \left(x', y'\right) ${:/}，{::nomarkdown}$ \begin{cases} x = \frac{x' - y'}{\sqrt{2}} \\ y = \frac{x' + y'}{\sqrt{2}} \end{cases} ${:/}

故 {::nomarkdown}$ 3\left(x'^2 + y'^2\right) - \left(x'^2 - y'^2\right) - 3\sqrt{2}\left(x' - y'\right) + \sqrt{2}\left(x' + y'\right) = -2 ${:/}

{::nomarkdown}$ \Leftrightarrow x'^2 - \sqrt{2}x' + 2y'^2 + 2\sqrt{2}y' + 1 = 0 \Leftrightarrow \left(x' - \frac{1}{\sqrt{2}}\right)^2 + 2\left(y' + \frac{1}{\sqrt{2}}\right)^2 = \frac{1}{2} ${:/}

故该曲线是椭圆

### 2.

设原坐标系中 {::nomarkdown}$ \left(x, y\right) ${:/} 在原坐标系逆时针旋转 {::nomarkdown}$ \frac{\pi}{4} ${:/} 所得坐标系中为 {::nomarkdown}$ \left(x', y'\right) ${:/}，{::nomarkdown}$ \begin{cases} x = \frac{x' - y'}{\sqrt{2}} \\ y = \frac{x' + y'}{\sqrt{2}} \end{cases} ${:/}

故 {::nomarkdown}$ x'^2 + y'^2 - 3\left(x'^2 - y'^2\right) + 4\sqrt{2}x' = 5 ${:/}

{::nomarkdown}$ \Leftrightarrow - 2\left(x' - \sqrt{2}\right)^2 + 4y'^2 = 1 ${:/}

故该曲线是双曲线

### 3.

{::nomarkdown}$ 2\left(x'^2 + y'^2\right) + 2\left(\cos \theta \sin \theta x'^2 + \left(\cos^2 \theta - \sin^2 \theta\right)x'y' - \cos \theta \sin \theta y'^2\right) = 1 ${:/}

{::nomarkdown}$ \Leftrightarrow \left(2 + \sin 2\theta\right)x'^2 + 2\cos 2\theta x'y' + \left(2 - \sin 2\theta\right)y'^2 = 1 ${:/}

故 {::nomarkdown}$ \begin{cases} \sin 2\theta = -1 \\ \cos 2\theta = 0 \end{cases} \Leftrightarrow 2\theta \in \left\{-\frac{\pi}{2}, \frac{3}{2}\pi\right\} \Leftrightarrow \theta \in \left\{-\frac{\pi}{4}, \frac{3}{4}\pi\right\} ${:/}

### 4.

{::nomarkdown}$ 3\left(x'^2 + y'^2\right) - 2\left(\cos \theta \sin \theta x'^2 + \left(\cos^2 \theta - \sin^2 \theta\right)x'y' - \cos \theta \sin \theta y'^2\right) = 1 ${:/}

{::nomarkdown}$ \Leftrightarrow \left(3 - \sin 2\theta\right)x'^2 - 2\cos 2\theta x'y' + \left(3 + \sin 2\theta\right)y'^2 = 1 ${:/}

{::nomarkdown}$ \cos 2\theta = 0 \Leftrightarrow 2\theta \in \left\{-\frac{3}{2}\pi, -\frac{\pi}{2}, \frac{\pi}{2}, \frac{3}{2}\pi\right\} ${:/}

{::nomarkdown}$ \theta \in \left\{-\frac{3}{4}\pi, \frac{\pi}{4}\right\}, 2x'^2 + 4y'^2 = 1 ${:/} 或 {::nomarkdown}$ \theta \in \left\{-\frac{\pi}{4}, \frac{3}{4}\pi\right\}, 4x'^2 + 2y'^2 = 1 ${:/}

### 5.

{::nomarkdown}$ \begin{aligned} & 7\left(\cos^2 \theta x'^2 - 2\cos \theta \sin \theta x'y' + \sin^2 \theta y'^2\right) \\ + & 2\sqrt{3}\left(\cos \theta \sin \theta x'^2 + \left(\cos^2 \theta - \sin^2 \theta\right)x'y' - \cos \theta \sin \theta y'^2\right) \\ + & 5\left(\sin^2 \theta x'^2 + 2\cos \theta \sin \theta x'y' + \cos^2 \theta y'^2\right) \\ = & 4 \end{aligned} ${:/}

{::nomarkdown}$ \Leftrightarrow \begin{aligned} & \left(7\frac{1 + \cos 2\theta}{2} + \sqrt{3}\sin 2\theta + 5\frac{1 - \cos 2\theta}{2}\right)x'^2 + \left(-7\sin 2\theta + 2\sqrt{3}\cos 2\theta + 5\sin 2\theta\right)x'y' \\ + & \left(7\frac{1 - \cos 2\theta}{2} - \sqrt{3}\sin 2\theta + 5\frac{1 + \cos 2\theta}{2}\right)y'^2 = 4 \end{aligned} ${:/}

{::nomarkdown}$ \Leftrightarrow \left(\cos 2\theta + \sqrt{3}\sin 2\theta + 6\right)x'^2 + 2\left(\sqrt{3}\cos 2\theta - \sin 2\theta\right)x'y' + \left(-\cos 2\theta - \sqrt{3}\sin 2\theta + 6\right)y'^2 = 4 ${:/}

{::nomarkdown}$ \cot2\theta = \frac{1}{\sqrt{3}} \Leftrightarrow 2\theta \in \left\{-\frac23\pi, \frac{\pi}{3}\right\} ${:/}

故可化得标准方程：{::nomarkdown}$ \theta = -\frac{\pi}{3}, x'^2 + 2y'^2 = 1 ${:/} 或 {::nomarkdown}$ \theta = \frac{\pi}{6}, 2x'^2 + y'^2 = 1 ${:/}

