* 函数 {::nomarkdown}$ f ${:/} 的定义域：{::nomarkdown}$ D\left(f\right) ${:/}，值域：{::nomarkdown}$ R\left(f\right) ${:/}，图象：{::nomarkdown}$ G\left(f\right) ${:/}

* 性质

  * 有界性：{::nomarkdown}$ f ${:/} 有上界、有下界、有界、无界，有界函数

  * 单调性：（严格）单调递增，（严格）单调递减

  * 奇偶性

  * 周期性

## 探究题

### 1.

* 若 {::nomarkdown}$ \lvert s - t \rvert \leqslant \frac{1}{2} ${:/}，{::nomarkdown}$ \lvert f\left(s\right) - f\left(t\right) \rvert < \lvert s - t \rvert \leqslant \frac{1}{2} ${:/}

* 若 {::nomarkdown}$ \lvert s - t \rvert > \frac{1}{2} ${:/}，不妨令 {::nomarkdown}$ s < t ${:/}，{::nomarkdown}$ \lvert f\left(s\right) - f\left(t\right) \rvert \overset{f\left(0\right) = f\left(1\right)}\leqslant \lvert f\left(s\right) - f\left(0\right) \rvert + \lvert f\left(1\right) - f\left(t\right) \rvert < \lvert s - 0 \rvert + \lvert 1 - t \rvert = 1 - \lvert s - t \rvert < \frac{1}{2} ${:/}

### 2.

* 若 {::nomarkdown}$ b \leqslant 0 ${:/}，{::nomarkdown}$ \begin{cases} \frac{13 - a^2}{2} = 2a \\ \frac{13-b^2}{2} = 2b \end{cases} \Rightarrow b > 0 ${:/}，舍

* 若 {::nomarkdown}$ a < 0 < b \land a + b \leqslant 0 ${:/}，{::nomarkdown}$ \begin{cases} \frac{13 - a^2}{2} = 2a \\ \frac{13 - 0^2}{2} = 2b \end{cases} \Leftrightarrow \begin{cases} a = -2 - \sqrt{17} \\ b = \frac{13}{4} \end{cases} ${:/}

* 若 {::nomarkdown}$ a < 0 < b \land a + b > 0 ${:/}，{::nomarkdown}$ \begin{cases} \frac{13 - 0^2}{2} = 2b \\ \frac{13 - b^2}{2} = 2a\end{cases} \Leftrightarrow \begin{cases} a = \frac{39}{32} \\ b = \frac{13}{4} \end{cases} ${:/}，舍

* 若 {::nomarkdown}$ a \geqslant 0 ${:/}，{::nomarkdown}$ \begin{cases} \frac{13 - a^2}{2} = 2b \\ \frac{13 - b^2}{2} = 2a \end{cases} \Leftrightarrow \begin{cases} a = 1 \\ b = 3 \end{cases} ${:/}

故 {::nomarkdown}$ \left[a, b\right] \in \left\{\left[-2 - \sqrt{17}, \frac{13}{4}\right], \left[1, 3\right]\right\} ${:/}

### 3.

{::nomarkdown}$ \begin{gathered} \forall x \in \left[-2, 2\right] \setminus \left[-1, 1\right] \cdot \\ \begin{aligned} \lvert f\left(x\right) \rvert & = \lvert x^2a + xb + c \rvert = \lvert \left(\frac{x^2}{2} - \frac{x}{2}\right)\left(a - b + c\right) + \left(-x^2 + 1\right)c + \left(\frac{x^2}{2} + \frac{x}{2}\right)\left(a + b + c\right) \rvert \\ & \leqslant \lvert \frac{x^2 - x}{2} \rvert \lvert f\left(-1\right) \rvert + \lvert -x^2 + 1 \rvert \lvert f\left(0\right) \rvert + \lvert \frac{x^2 + x}{2} \rvert \lvert f\left(1\right) \rvert \leqslant \frac{x^2 - x}{2} + \left(x^2 - 1\right) + \frac{x^2 + x}{2} \\ & = 2x^2 - 1 \leqslant 7 \end{aligned} \end{gathered} ${:/}

### 4.

设 {::nomarkdown}$ P\left(x\right) = ax^2 + bx + c ${:/}，若满足（1），{::nomarkdown}$ \lvert P\left(-1\right) \rvert, \lvert P\left(0\right) \rvert, \lvert P\left(1\right) \rvert \leqslant 1 ${:/}

则 {::nomarkdown}$ \begin{aligned} \lvert P\left(2\right) \rvert & = \lvert \left(a - b + c\right) - 3c + 3\left(a + b + c\right) \rvert \\ & \leqslant \lvert P\left(-1\right) \rvert + 3 \lvert P\left(0\right) \rvert + 3 \lvert P\left(1\right) \rvert \\ & \leqslant 7 < 8 \end{aligned} ${:/}，不满足（2）

故不存在这样的 {::nomarkdown}$ P\left(x\right) ${:/}

### 5.

① {::nomarkdown}$ n = 1 ${:/} 时，{::nomarkdown}$ f\left(2^1\right) = 2^1 ${:/}

② 假设 {::nomarkdown}$ n = k ${:/} 时，{::nomarkdown}$ f\left(2^k\right) = 2^k ${:/}，{::nomarkdown}$ n = k + 1 ${:/} 时，

　 {::nomarkdown}$ f\left(2^{k + 1}\right) = f\left(2\right)f\left(2^k\right) = 2^{k + 1} ${:/}

由 ①②，{::nomarkdown}$ \forall n \cdot f\left(2^n\right) = 2^n ${:/}

{::nomarkdown}$ f\left(1 \times 1\right) = f\left(1\right)f\left(1\right) \Rightarrow f\left(1\right) = 1 ${:/}

{::nomarkdown}$ \forall n > 1 \cdot ${:/} 设 {::nomarkdown}$ n \in \left[2^k, 2^{k + 1}\right) ${:/}

{::nomarkdown}$ 2^{k + 1} = f\left(2^{k + 1}\right) \geqslant f\left(2^{k + 1} - 1\right) + 1 \geqslant \cdots \geqslant f\left(2^k + 1\right) + 2^k - 1 \geqslant f\left(2^k\right) + 2^k = 2^{k + 1} ${:/}

故 {::nomarkdown}$ f\left(2^{k + 1} - 1\right) + 1 = \cdots = f\left(2^k + 1\right) + 2^k - 1 = f\left(2^k\right) + 2^k = 2^{k + 1} ${:/}

{::nomarkdown}$ \Rightarrow \forall m \in \left[2^k, 2^{k + 1}\right) \cdot f\left(m\right) = m ${:/}

{::nomarkdown}$ \Rightarrow f\left(n\right) = n ${:/}

