* 零复数

## 探究题

### 1.

设 {::nomarkdown}$ z = r\e^{\i\theta} \enspace \left(r > 0, \theta \in \left[0, 2\pi\right)\right) ${:/}

则 {::nomarkdown}$ r^3\e^{\i \cdot 3\theta} = 8\e^{\i\pi} \Leftrightarrow \begin{cases} r^3 = 8 \\ \exists k \in \Z \cdot 3\theta - \pi = 2k\pi \end{cases} \Leftrightarrow \begin{cases} r = 2 \\ \theta \in \left\{\frac{\pi}{3}, \pi, \frac{5}{3}\pi\right\} \end{cases} ${:/}

故 {::nomarkdown}$ z \in \left\{1 + \sqrt{3}\i, -2, 1 - \sqrt{3}\i\right\} ${:/}

### 2.

令 {::nomarkdown}$ \begin{cases} a = \lvert z_1 - z_2 \rvert \lvert z_3 - z_4 \rvert \\ b = \lvert z_1 - z_3 \rvert \lvert z_2 - z_4 \rvert \\ c =
\lvert z_1 - z_4 \rvert \lvert z_2 - z_3 \rvert \end{cases} ${:/}

由托勒密定理，{::nomarkdown}$ \left(a + b - c\right)\left(b + c - a\right)\left(c + a - b\right) = 0 ${:/}

### 3.

* 若 {::nomarkdown}$ \lvert \cos \theta \rvert = 1 ${:/}，{::nomarkdown}$ \lvert z \rvert = 1, z = \cos \theta ${:/}

* 若 {::nomarkdown}$ \lvert \cos \theta \rvert < 1 ${:/}，{::nomarkdown}$ z \notin \R ${:/}，设 {::nomarkdown}$ z = a + b\i \enspace \left(b \neq 0\right) ${:/}

  则 {::nomarkdown}$ a + b\i + \frac{a - b\i}{a^2 + b^2} = 2\cos \theta \Leftrightarrow \begin{cases} a^2 + b^2 = 1 \\ a = \cos \theta \end{cases} \Leftrightarrow z \in \left\{\cos \theta + \left(\sin \theta\right)\i, \cos \left(-\theta\right) + \left(\sin \left(-\theta\right)\right)\i\right\} ${:/}


{::nomarkdown}$ \Rightarrow \begin{cases} \lvert z^n \rvert = 1 \\ \Ree\left(z^n\right) = \cos n\theta \end{cases} \Rightarrow z^n + \frac{1}{z^n} = z^n + \overline{z^n} = 2\Ree\left(z^n\right) = 2\cos n\theta ${:/}

### 4.

{::nomarkdown}$ f\left(x\right) = f\left(-x\right) \Leftrightarrow -\log_3 \left(3^x + 1\right) + abx = -\log_3 \frac{3^x + 1}{3^x} \Leftrightarrow abx = x ${:/}

{::nomarkdown}$ g\left(x\right) + g\left(-x\right) = 0 \Leftrightarrow 2^x + \left(a + b\right)2^{-x} + 2^{-x} + \left(a + b\right)2^x = 0 \Leftrightarrow \left(a + b + 1\right)\left(2^x + 2^{-x}\right) = 0 ${:/}

故 {::nomarkdown}$ a, b ${:/} 是 {::nomarkdown}$ x^2 + x + 1 = 0 ${:/} 的两根

{::nomarkdown}$ x^2 + x + 1 = 0 \Rightarrow x^3 = 1 ${:/}

故原式 {::nomarkdown}$ = a + b = -1 ${:/}

### 5.

{::nomarkdown}$ \alpha = \overline \beta ${:/}，令 {::nomarkdown}$ \lvert \alpha \rvert = r = \lvert \beta \rvert ${:/}

{::nomarkdown}$ \omega := \e^{\i \cdot \frac{2}{3}\pi}, \omega^3 = 1, 1 + \omega + \omega^2 = 0 ${:/}

{::nomarkdown}$ \frac{\alpha^2}{\beta} \in \R \Leftrightarrow \frac{\alpha^3}{r^2} \in \R \Leftrightarrow \alpha \in \left\{r\omega, r\omega^2\right\} ${:/}

{::nomarkdown}$ \frac{\alpha}{\beta} = \frac{\alpha^2}{r^2} \in \left\{\omega, \omega^2\right\} ${:/}

{::nomarkdown}$ 3 \mid 5985 ${:/}，故原式 {::nomarkdown}$ = 0 ${:/}

